src/State.v
@@ -1,314 +1,91 @@
 From RecordUpdate Require Import RecordSet.
-Import RecordSetNotations.
-Require Common Condition Memory Instruction CodeStorage.
+Require Common Condition Ergs Memory Instruction CodeStorage ExecutionStack.
 
-Import ZArith Condition Common MemoryBase Memory CodeStorage Instruction ZMod List ListNotations.
+Import ZArith Condition Common Ergs ExecutionStack MemoryBase Memory CodeStorage Instruction ZMod List.
+Import ListNotations RecordSetNotations.
 
-
-Definition mem_page := mem_page instruction_predicated instruction_invalid.
+Definition page := page instruction_predicated instruction_invalid.
+Definition code_manager := code_manager instruction_predicated instruction_invalid.
 
 Definition exception_handler := code_address.
 
-Definition ergs := u32.
-
-Record callframe_common := mk_cf {
-                               cf_exception_handler_location: exception_handler;
-                               cf_sp: stack_address;
-                               cf_pc: code_address;
-                               cf_ergs_remaining: ergs;
-                             }.
-#[export] Instance etaCFC : Settable _ :=
-  settable! mk_cf < cf_exception_handler_location; cf_sp; cf_pc; cf_ergs_remaining >.
-
-Record callframe_external :=
-  mk_extcf {
-      ecf_this_address: contract_address;
-      ecf_msg_sender: contract_address;
-      ecf_code_address: code_address; (* TODO check *)
-      ecf_mem_context: ctx_mem_pages;
-      ecf_is_static: bool; (** forbid any write-like "logs" and so state modifications, event emissions, etc *)
-      ecf_context_u128_value: u128;
-      ecf_saved_storage_state: storage_type;
-      ecx_common :> callframe_common
-    }.
-
-#[export] Instance etaCFE : Settable _ :=
-  settable! mk_extcf <
-      ecf_this_address;
-      ecf_msg_sender;
-      ecf_code_address;
-      ecf_mem_context;
-      ecf_is_static;
-      ecf_context_u128_value;
-      ecf_saved_storage_state;
-      ecx_common>.
-
-Inductive execution_frame :=
-| InternalCall (_: callframe_common) (tail: execution_frame): execution_frame
-| ExternalCall (_: callframe_external) (tail: option execution_frame): execution_frame.
-
-Definition cfc (ef: execution_frame) : callframe_common :=
-  match ef with
-  | InternalCall x _ => x
-  | ExternalCall x _ => x
-  end.
-
-Definition cfc_map (f:callframe_common->callframe_common) (ef: execution_frame) : execution_frame :=
-  match ef with
-  | InternalCall x tail => InternalCall (f x) tail
-  | ExternalCall x tail => ExternalCall (x <| ecx_common ::= f |>) tail
-  end.
-
-Definition active_exception_handler (ef: execution_frame) : exception_handler :=
-  (cfc ef).(cf_exception_handler_location).
-
-Definition ergs_remaining (ef:execution_frame) : ergs := (cfc ef).(cf_ergs_remaining).
-Definition ergs_map (f: ergs->ergs) (ef:execution_frame) : execution_frame
-  := cfc_map (fun x => x <| cf_ergs_remaining ::= f |>) ef.
-
-Definition ergs_set newergs := ergs_map (fun _ => newergs).
-
-Inductive ergs_reimburse : ergs -> execution_frame -> execution_frame -> Prop :=
-  | er_reimburse: forall delta new_ergs ef ef',
-      delta + ergs_remaining ef = (new_ergs, false) ->
-      ef' = ergs_set new_ergs ef ->
-      ergs_reimburse delta ef ef'.
-
-
-Inductive ergs_reimburse_caller : execution_frame -> execution_frame -> Prop
-  :=
-  |erc_internal: forall caller new_caller cf,
-      ergs_reimburse (ergs_remaining (InternalCall cf caller)) caller
-        new_caller ->
-      ergs_reimburse_caller (InternalCall cf caller) new_caller
-  |erc_external: forall caller new_caller cf,
-      ergs_reimburse (ergs_remaining (ExternalCall cf (Some caller))) caller
-        new_caller ->
-      ergs_reimburse_caller (ExternalCall cf (Some caller)) new_caller.
-
-Definition ergs_zero := ergs_set zero32.
-
-(** Fetching value of the stack pointer itself. *)
-Inductive fetch_sp : execution_frame -> stack_address -> Prop :=
-| fsp_fetch_ext:
-  forall (cf:callframe_external) tail (sp_value:stack_address),
-    cf_sp cf = sp_value ->
-    fetch_sp (ExternalCall cf tail) sp_value
-| fsp_fetch_int:
-  forall (cf:callframe_common) tail (sp_value:stack_address),
-    cf_sp cf = sp_value ->
-    fetch_sp (InternalCall cf tail) sp_value
-.
-
-Inductive update_sp_cfc : stack_address -> callframe_common -> callframe_common
-                          -> Prop :=
-  | usc_update:
-    forall ehl sp pc ergs sp',
-      update_sp_cfc sp' (mk_cf ehl sp pc ergs) (mk_cf ehl sp' pc ergs).
-
-Inductive update_sp_extcall: stack_address -> callframe_external -> callframe_external
-                          -> Prop :=
-  | usce_update:
-    forall sp' cf cf' this_address msg_sender code_address mem_context is_static context_u128_value saved_storage_state cfc,
-      update_sp_cfc sp' cf cf' ->
-      update_sp_extcall sp'
-        (mk_extcf this_address msg_sender code_address mem_context is_static
-           context_u128_value saved_storage_state cfc)
-        (mk_extcf this_address msg_sender code_address mem_context is_static
-           context_u128_value saved_storage_state cf')
-       .
-
-Inductive update_sp : stack_address -> execution_frame -> execution_frame -> Prop :=
-| usp_ext:
-  forall ecf ecf' tail sp',
-    update_sp_extcall sp' ecf ecf' ->
-    update_sp sp' (ExternalCall ecf tail) (ExternalCall ecf' tail)
-| usp_int:
-  forall sp' cf cf' tail,
-    update_sp_cfc sp' cf cf' ->
-    update_sp sp' (InternalCall cf tail) (InternalCall cf' tail).
-
-
-(** Fetching value of the program counter itself. *)
-Inductive fetch_pc : execution_frame -> code_address -> Prop :=
-| fpc_fetch_ext:
-  forall addr sender ca mc st ctx ss eh sa tail ergs (pc_value:code_address),
-    fetch_pc (ExternalCall (mk_extcf addr sender ca mc st ctx ss
-                              (mk_cf eh sa pc_value ergs) ) tail) pc_value
-| fpc_fetch_int:
-  forall eh sa ergs tail (pc_value:code_address),
-    fetch_pc (InternalCall (mk_cf eh sa pc_value ergs) tail) pc_value
-.
-
-Definition pc_get (ef: execution_frame) : code_address :=
-  match ef with
-  | InternalCall cf _ => cf.(cf_pc)
-  | ExternalCall ef tail => ef.(ecx_common).(cf_pc)
-  end.
-
-Definition sp_get (ef: execution_frame) : stack_address :=
-  match ef with
-  | InternalCall cf _ => cf.(cf_sp)
-  | ExternalCall ef tail => ef.(ecx_common).(cf_sp)
-  end.
-
-Definition pc_mod f ef :=
-  match ef with
-  | InternalCall x tail => InternalCall (x <| cf_pc ::=  f |>) tail
-  | ExternalCall x tail => ExternalCall (x <| ecx_common ::= fun cf => cf <| cf_pc ::=  f |> |>) tail
-  end.
-
-Definition sp_mod (f:stack_address->stack_address) ef :=
-  match ef with
-  | InternalCall x tail => InternalCall (x <| cf_sp ::=  f |>) tail
-  | ExternalCall x tail => ExternalCall (x <| ecx_common ::= fun cf => cf <| cf_sp ::=  f |> |>) tail
-  end.
-
-Definition pc_inc := pc_mod (fun oldpc => fst (uinc_overflow _ oldpc)).
-Definition pc_set new := pc_mod (fun _ => new).
-
-Theorem pc_get_correct:
-  forall ef, fetch_pc ef (pc_get ef).
-Proof.
-  intros [ []|[] ]; simpl; [|destruct ecx_common0]; constructor.
-Qed.
-
-Inductive update_pc_cfc : code_address -> callframe_common -> callframe_common
-                          -> Prop :=
-  | upc_update:
-    forall ehl sp ergs pc pc',
-      update_pc_cfc pc' (mk_cf ehl sp pc ergs) (mk_cf ehl sp pc' ergs).
-
-Inductive update_pc_extcall: code_address -> callframe_external -> callframe_external
-                          -> Prop :=
-  | upe_update:
-    forall pc' cf cf' this_address msg_sender code_address mem_context is_static context_u128_value saved_storage_state,
-      update_pc_cfc pc' cf cf' ->
-      update_pc_extcall pc'
-        (mk_extcf this_address msg_sender code_address mem_context is_static
-           context_u128_value saved_storage_state cf)
-        (mk_extcf this_address msg_sender code_address mem_context is_static
-           context_u128_value saved_storage_state cf')
-       .
-
-Inductive update_pc : code_address -> execution_frame -> execution_frame -> Prop :=
-| upc_ext:
-  forall ecf ecf' tail pc',
-    update_pc_extcall pc' ecf ecf' ->
-    update_pc pc' (ExternalCall ecf tail) (ExternalCall ecf' tail)
-| upc_int:
-  forall pc' cf cf' tail,
-    update_pc_cfc pc' cf cf' ->
-    update_pc pc' (InternalCall cf tail) (InternalCall cf' tail).
-
-Theorem update_pc_correct:
-  forall ef pc, update_pc pc ef (pc_set pc ef).
-Proof.
-  intros [ []|[] ] pc; simpl; [|destruct ecx_common0]; repeat constructor.
-Qed.
-
-
-Fixpoint topmost_extframe (ef : execution_frame) : callframe_external :=
-  match ef with
-  | InternalCall _ tail => topmost_extframe tail
-  | ExternalCall x tail => x
-  end.
-
-(* Inductive topmost_extframe : execution_frame -> execution_frame -> Prop := *)
-(* | te_Top: forall x t, topmost_extframe (ExternalCall x t) (ExternalCall x t) *)
-(* | te_Deeper: forall c t f, *)
-(*     topmost_extframe t f -> topmost_extframe (InternalCall c t) f *)
-(* . *)
-
 Definition KERNEL_MODE_MAXADDR : contract_address := int_mod_of _ (2^16-1).
+
+
+Section AllocatedPages.
+  Import Bool Nat.
+
+  Definition pages : Type := list (page_id * page).
+
+  Inductive page_replace:  page_id -> page -> pages -> pages -> Prop :=
+  | mm_replace_base: forall oldpage id newpage tail,
+      page_replace id newpage ((id, oldpage)::tail) ((id,newpage)::tail)
+  | mm_replace_ind: forall oldpage id not_id newpage tail tail',
+      page_replace id newpage tail tail' ->
+      id <> not_id ->
+      page_replace id newpage ((not_id,oldpage)::tail) ((not_id,oldpage)::tail').
+
+  Inductive page_has_id : pages -> page_id -> page -> Prop :=
+  | mpid_select : forall mm id page,
+      List.In (id, page) mm ->
+      page_has_id mm id page.
+
+  Definition is_active_page (ef:callframe) (id: page_id) : bool :=
+    eqb (active_code_id ef) id ||
+      eqb (active_stack_id ef) id ||
+      eqb (active_const_id ef) id ||
+      eqb (active_heap_id ef) id ||
+      eqb (active_auxheap_id ef) id .
+
+    Inductive active_codepage : pages -> callframe -> page -> Prop :=
+    | ap_active_code: forall mm ef codepage,
+        page_has_id mm (active_code_id ef) codepage ->
+        active_codepage mm ef codepage.
+
+    Inductive active_constpage : pages -> callframe -> page -> Prop :=
+    | ap_active_const: forall mm ef constpage,
+        page_has_id mm (active_const_id ef) constpage ->
+        active_constpage mm ef constpage.
+
+    Inductive active_stackpage : pages -> callframe -> page -> Prop :=
+    | ap_active_stack: forall mm ef stackpage,
+        page_has_id mm (active_stack_id ef) stackpage ->
+        active_stackpage mm ef stackpage.
+
+    Inductive active_heappage : pages -> callframe -> page -> Prop :=
+    | ap_active_heap: forall mm ef heappage,
+        page_has_id mm (active_heap_id ef) heappage ->
+        active_heappage mm ef heappage.
+
+    Inductive active_auxheappage : pages -> callframe -> page -> Prop :=
+    | ap_active_auxheap: forall mm ef auxheappage,
+        page_has_id mm (active_auxheap_id ef) auxheappage ->
+        active_auxheappage mm ef auxheappage.
+
+End AllocatedPages.
+
+
+Definition update_memory_context (ps:active_pages): callframe -> callframe :=
+ change_topmost_extframe (fun ef => ef <| ecf_pages := ps |> ).
+
 
 Definition addr_is_kernel (addr:contract_address) : bool :=
   lt_unsigned _ addr KERNEL_MODE_MAXADDR.
 
-Definition is_kernel (ef:execution_frame) : bool :=
+Definition is_kernel (ef:callframe) : bool :=
   let ef := topmost_extframe ef in
   addr_is_kernel ef.(ecf_this_address).
 
-Definition mem_manager := list (mem_page_id * mem_page).
 
-Inductive mem_page_replace: mem_manager -> mem_page_id -> mem_page -> mem_manager -> Prop :=
- | mm_replace: forall mm h t id page mm' oldpage,
-     mm = h ++ (id, oldpage) :: t ->
-     mm' = h ++ (id, page)::t ->
-     mem_page_replace mm id page mm'.
-
-Record global_state := {
+Record state := mk_state {
     gs_flags : flags_state;
     gs_regs: regs_state;
-    gs_storages: contract_collection_type;
-    gs_contract_code: code_manager instruction_predicated instruction_invalid;
-    (* gs_pending_exception: bool; we can probably store optional here *)
-    gs_mem_pages: mem_manager ;
-    gs_callstack: execution_frame;
+    gs_depot: depot;
+    gs_contracts: code_manager;
+    gs_pages: pages;
+    gs_callstack: execution_stack;
     gs_context_u128: u128;
   }.
-#[export] Instance etaXGS : Settable _ := settable! Build_global_state <gs_flags ; gs_regs; gs_storages; gs_contract_code; gs_mem_pages; gs_callstack; gs_context_u128>.
+#[export] Instance etaXGS : Settable _ := settable! mk_state <gs_flags ; gs_regs; gs_depot; gs_contracts; gs_pages; gs_callstack; gs_context_u128>.
 
 
-
-Definition active_mem_ctx (ef: execution_frame) : ctx_mem_pages :=
-  (topmost_extframe ef).(ecf_mem_context).
-
-Inductive mem_page_by_id : mem_manager -> mem_page_id
-                           -> mem_page -> Prop :=
-| mpid_select : forall mm id page,
-    List.In (id, page) mm ->
-    mem_page_by_id mm id page
-.
-
-
-
-Definition active_code_id (ef: execution_frame) : mem_page_id :=
-  (active_mem_ctx ef).(ctx_code_page_id).
-
-Definition active_stack_id (ef: execution_frame) : mem_page_id :=
-  (active_mem_ctx ef).(ctx_stack_page_id).
-
-Definition active_const_id (ef: execution_frame) : mem_page_id :=
-  (active_mem_ctx ef).(ctx_const_page_id).
-
-Definition active_heap_id (ef: execution_frame) : mem_page_id :=
-  (active_mem_ctx ef).(ctx_heap_page_id).
-
-Definition active_auxheap_id (ef: execution_frame) : mem_page_id :=
-  (active_mem_ctx ef).(ctx_heap_aux_page_id).
-
-
-Import Bool Nat.
-
-Definition active_page (ef:execution_frame) (id: mem_page_id) : bool :=
-  eqb (active_code_id ef) id ||
-    eqb (active_stack_id ef) id ||
-    eqb (active_const_id ef) id ||
-    eqb (active_heap_id ef) id ||
-    eqb (active_auxheap_id ef) id .
-
- Inductive active_codepage : mem_manager -> execution_frame -> mem_page -> Prop :=
- | ap_active_code: forall mm ef codepage,
-     mem_page_by_id mm (active_code_id ef) codepage ->
-     active_codepage mm ef codepage.
-
- Inductive active_constpage : mem_manager -> execution_frame -> mem_page -> Prop :=
- | ap_active_const: forall mm ef constpage,
-     mem_page_by_id mm (active_const_id ef) constpage ->
-     active_constpage mm ef constpage.
-
- Inductive active_stackpage : mem_manager -> execution_frame -> mem_page -> Prop :=
- | ap_active_stack: forall mm ef stackpage,
-     mem_page_by_id mm (active_stack_id ef) stackpage ->
-     active_stackpage mm ef stackpage.
-
- Inductive active_heappage : mem_manager -> execution_frame -> mem_page -> Prop :=
- | ap_active_heap: forall mm ef heappage,
-     mem_page_by_id mm (active_heap_id ef) heappage ->
-     active_heappage mm ef heappage.
-
- Inductive active_auxheappage : mem_manager -> execution_frame -> mem_page -> Prop :=
- | ap_active_auxheap: forall mm ef auxheappage,
-     mem_page_by_id mm (active_auxheap_id ef) auxheappage ->
-     active_auxheappage mm ef auxheappage.
