src/CodeStorage.v
@@ -10,9 +10,9 @@ Definition DEPLOYER_SYSTEM_CONTRACT_ADDRESS : contract_address
 Section Defs.
   Variable ins_type: Type.
   Variable invalid_ins: ins_type.
-  
+
   Let code_page := code_page ins_type invalid_ins.
-  
+
   Definition code_storage_params := {|
                                      addressable_block := code_page;
                                      address_bits := 256;
@@ -30,10 +30,10 @@ Section Defs.
 
 
   Definition is_fresh cm := contains _ VersionedHash.eq_dec (cm_fresh cm).
-  
-  Inductive code_fetch: contract_collection_type -> code_storage
+
+  Inductive code_fetch: depot -> code_storage
                         -> contract_address -> (versioned_hash *code_page * code_length) -> Prop :=
-  | cfh_load : forall (contracts:contract_collection_type) (called_address:contract_address) deployer_storage hash_enc (code_storage:code_storage) code_length_in_words extra_marker partial_hash page_init,
+  | cfh_load : forall (contracts:depot) (called_address:contract_address) deployer_storage hash_enc (code_storage:code_storage) code_length_in_words extra_marker partial_hash page_init,
       load_result _ DEPLOYER_SYSTEM_CONTRACT_ADDRESS contracts deployer_storage ->
       load_result storage_params (@resize _ 256 called_address) deployer_storage hash_enc ->
       hash_enc <> zero256 ->
@@ -42,9 +42,9 @@ Section Defs.
       load_result (code_storage_params) (@resize _ 256 partial_hash) code_storage page_init ->
       code_fetch contracts code_storage called_address ((mk_vhash code_length_in_words extra_marker partial_hash), page_init,code_length_in_words)
 
-  | cfh_load_aa_default : forall (contracts:contract_collection_type) (called_address:contract_address) deployer_storage (code_storage:code_storage),
+  | cfh_load_aa_default : forall (contracts:depot) (called_address:contract_address) deployer_storage (code_storage:code_storage),
       load_result _ DEPLOYER_SYSTEM_CONTRACT_ADDRESS contracts deployer_storage ->
       load_result storage_params (@resize _ 256 called_address) deployer_storage zero256->
       code_fetch contracts code_storage called_address (DEFAULT_AA_VHASH, DEFAULT_AA_CODE _ invalid_ins,code_length_in_words DEFAULT_AA_VHASH).
-  
+
 End Defs.
