src/FarCalls.v
@@ -1,7 +1,7 @@
 From RecordUpdate Require Import RecordSet.
-Require Common Condition Memory Instruction State MemoryOps ABI SemanticCommon.
+Require Common Ergs Condition ExecutionStack Memory Instruction State MemoryOps ABI SemanticCommon.
 
-Import Bool ZArith Common CodeStorage Condition MemoryBase Memory MemoryOps
+Import Bool ZArith Common CodeStorage Condition Ergs ExecutionStack MemoryBase Memory MemoryOps
   Instruction State SemanticCommon ZMod
   ABI ABI.FarCall ABI.Ret ABI.NearCall ABI.FatPointer Arg Arg.Coercions RecordSetNotations.
 Import List ListNotations.
@@ -20,7 +20,7 @@ Record FarCallExceptions : Set := {
   }.
 
 Definition code_storage := code_storage _ instruction_invalid.
-Definition code_manager := code_manager _ instruction_invalid.
+Definition code_manager := code_manager.
 
 Inductive decommitment_cost (cm:code_manager) vhash (code_length_in_words: code_length): ergs -> Prop :=
   |dc_fresh: forall cost,
@@ -31,9 +31,7 @@ Inductive decommitment_cost (cm:code_manager) vhash (code_length_in_words: code_
     is_fresh _ _ cm vhash = false ->
     decommitment_cost cm vhash code_length_in_words zero32.
 
-
-
-Inductive alloc_pages_extframe:  mem_manager -> ctx_mem_pages -> code_page -> mem_manager * ctx_mem_pages -> Prop :=
+Inductive alloc_pages_extframe:  pages -> active_pages -> code_page -> pages * active_pages -> Prop :=
   | ape_alloc: forall code mm ctx code_id const_id stack_id heap_id heap_aux_id,
       alloc_pages_extframe mm ctx code
      ( (heap_aux_id, (DataPage _ _ (empty _)))::
@@ -46,12 +44,12 @@ Inductive alloc_pages_extframe:  mem_manager -> ctx_mem_pages -> code_page -> me
          ctx_const_page_id := const_id;
          ctx_stack_page_id := stack_id;
          ctx_heap_page_id := heap_id;
-         ctx_heap_aux_page_id := heap_aux_id;
+         ctx_auxheap_page_id := heap_aux_id;
          ctx_heap_bound := NEW_FRAME_MEMORY_STIPEND;
          ctx_aux_heap_bound := NEW_FRAME_MEMORY_STIPEND;
        |} ).
 
-Inductive grow_page: forward_page_type -> mem_address -> ctx_mem_pages -> ctx_mem_pages -> Prop :=
+Inductive grow_page: forward_page_type -> mem_address -> active_pages -> active_pages -> Prop :=
   | gp_heap: forall code_id const_id stack_id heap_id heap_aux_id heap_bound
                aux_heap_bound new_bound diff,
       heap_bound + diff = (new_bound, false) ->
@@ -61,7 +59,7 @@ Inductive grow_page: forward_page_type -> mem_address -> ctx_mem_pages -> ctx_me
          ctx_const_page_id := const_id;
          ctx_stack_page_id := stack_id;
          ctx_heap_page_id := heap_id;
-         ctx_heap_aux_page_id := heap_aux_id;
+         ctx_auxheap_page_id := heap_aux_id;
          ctx_heap_bound := heap_bound;
          ctx_aux_heap_bound := aux_heap_bound;
        |}
@@ -70,7 +68,7 @@ Inductive grow_page: forward_page_type -> mem_address -> ctx_mem_pages -> ctx_me
          ctx_const_page_id := const_id;
          ctx_stack_page_id := stack_id;
          ctx_heap_page_id := heap_id;
-         ctx_heap_aux_page_id := heap_aux_id;
+         ctx_auxheap_page_id := heap_aux_id;
          ctx_heap_bound := new_bound;
          ctx_aux_heap_bound := aux_heap_bound;
        |}
@@ -83,7 +81,7 @@ Inductive grow_page: forward_page_type -> mem_address -> ctx_mem_pages -> ctx_me
          ctx_const_page_id := const_id;
          ctx_stack_page_id := stack_id;
          ctx_heap_page_id := heap_id;
-         ctx_heap_aux_page_id := heap_aux_id;
+         ctx_auxheap_page_id := heap_aux_id;
          ctx_heap_bound := heap_bound;
          ctx_aux_heap_bound := aux_heap_bound;
        |}
@@ -92,49 +90,52 @@ Inductive grow_page: forward_page_type -> mem_address -> ctx_mem_pages -> ctx_me
          ctx_const_page_id := const_id;
          ctx_stack_page_id := stack_id;
          ctx_heap_page_id := heap_id;
-         ctx_heap_aux_page_id := heap_aux_id;
+         ctx_auxheap_page_id := heap_aux_id;
          ctx_heap_bound := heap_bound;
          ctx_aux_heap_bound := new_bound;
        |}.
 
-Inductive code_fetch_and_pay : contract_collection_type -> code_manager -> contract_address
-                               -> execution_frame -> execution_frame * code_page
+Inductive code_fetch_and_pay : depot -> code_manager -> contract_address
+                               -> execution_stack -> execution_stack * code_page
                                ->Prop :=
 | cfp_apply:
-  forall storages codes (dest_addr: contract_address) vhash dest_addr new_code_page code_length
+  forall depot codes (dest_addr: contract_address) vhash dest_addr new_code_page code_length
     cost__decomm xstack0 xstack1,
-    code_fetch _ _ storages codes.(cm_storage _ _) dest_addr (vhash, new_code_page, code_length) ->
+    code_fetch _ _ depot codes.(cm_storage _ _) dest_addr (vhash, new_code_page, code_length) ->
     decommitment_cost codes vhash code_length cost__decomm ->
     pay cost__decomm xstack0 xstack1 ->
-    code_fetch_and_pay storages codes dest_addr xstack0 (xstack1, new_code_page).
+    code_fetch_and_pay depot codes dest_addr xstack0 (xstack1, new_code_page).
 
 Definition max_passable (remaining:ergs) : ergs :=
     int_mod_of _(((int_val _ remaining) / 64 ) * 63)%Z.
 
-Inductive pass_allowed_ergs : ergs -> ergs -> execution_frame -> execution_frame -> Prop :=
+Inductive pass_allowed_ergs : ergs -> ergs -> execution_stack -> execution_stack -> Prop :=
   | pae_apply: forall xstack1 xstack2 pass_ergs_query,
   let pass_ergs_actual := ZMod.min _ (max_passable (ergs_remaining xstack1)) pass_ergs_query in
   pay pass_ergs_actual xstack1 xstack2 ->
   pass_allowed_ergs pass_ergs_query pass_ergs_actual xstack1 xstack2.
 
-Inductive step_farcall: instruction -> global_state -> global_state -> Prop :=
 
-|step_FarCall_NonKernel_Forward: forall flags regs mem_pages xstack0 xstack1 xstack2
-                                   (handler:imm_in) handler_location storages
+
+(* Not implemented: shards *)
+Inductive step_farcall: instruction -> state -> state -> Prop :=
+
+|step_FarCall_NonKernel_Forward: forall flags regs pages xstack0 xstack1 xstack2
+                                   (handler:imm_in) handler_location depot
                                    codes context_u128 (abi dest:in_reg)
-                                   is_static new_mem_pages
+                                   is_static new_pages
                                    new_code_page (dest_val:word_type)
                                    abi_val
                                    new_mem_ctx in_ptr shrunk_ptr shard_id
                                    pass_ergs_query pass_ergs_actual vtag,
 
     let old_extframe := topmost_extframe xstack0 in
-    let old_mem_ctx  := old_extframe.(ecf_mem_context) in
+    let old_mem_ctx  := old_extframe.(ecf_pages) in
     let current_contract := old_extframe.(ecf_this_address) in
 
-    resolve_fetch_value regs xstack0 mem_pages dest (mk_pv vtag dest_val) ->
-    resolve_fetch_value regs xstack0 mem_pages abi (PtrValue abi_val) ->
-    resolve_fetch_value regs xstack0 mem_pages handler (IntValue handler_location) ->
+    resolve_fetch_value regs xstack0 pages dest (mk_pv vtag dest_val) ->
+    resolve_fetch_value regs xstack0 pages abi (PtrValue abi_val) ->
+    resolve_fetch_value regs xstack0 pages handler (IntValue handler_location) ->
     let dest_addr := resize _ 160 dest_val in
     addr_is_kernel dest_addr = false ->
 
@@ -150,9 +151,9 @@ Inductive step_farcall: instruction -> global_state -> global_state -> Prop :=
 
     fat_ptr_shrink in_ptr shrunk_ptr ->
 
-    code_fetch_and_pay storages codes dest_addr xstack0 (xstack1, new_code_page) ->
+    code_fetch_and_pay depot codes dest_addr xstack0 (xstack1, new_code_page) ->
 
-    alloc_pages_extframe mem_pages old_mem_ctx new_code_page (new_mem_pages, new_mem_ctx) ->
+    alloc_pages_extframe pages old_mem_ctx new_code_page (new_pages, new_mem_ctx) ->
 
     pass_allowed_ergs pass_ergs_query pass_ergs_actual xstack1 xstack2 ->
 
@@ -162,11 +163,11 @@ Inductive step_farcall: instruction -> global_state -> global_state -> Prop :=
                          ecf_this_address := dest_addr;
                          ecf_msg_sender := current_contract;
                          ecf_code_address := zero16;
-                         ecf_mem_context := new_mem_ctx;
+                         ecf_pages := new_mem_ctx;
                          ecf_is_static :=  ecf_is_static old_extframe || is_static;
                          ecf_context_u128_value := context_u128;
-                         ecf_saved_storage_state := load _ current_contract storages;
-                         ecx_common := {|
+                         ecf_saved_storage_state := load _ current_contract depot;
+                         ecf_common := {|
                                         cf_exception_handler_location := resize _ code_address_bits handler_location;
                                         cf_sp := INITIAL_SP_ON_FAR_CALL;
                                         cf_pc := zero16;
@@ -177,32 +178,32 @@ Inductive step_farcall: instruction -> global_state -> global_state -> Prop :=
              {|
                gs_flags        := flags;
                gs_regs         := regs;
-               gs_mem_pages    := mem_pages;
+               gs_pages    := pages;
                gs_callstack    := xstack0;
                gs_context_u128 := context_u128;
 
 
-               gs_storages     := storages;
-               gs_contract_code:= codes;
+               gs_depot     := depot;
+               gs_contracts    := codes;
              |}
              {|
                gs_flags        := flags_clear;
                gs_regs         := new_regs;
-               gs_mem_pages    := new_mem_pages;
+               gs_pages    := new_pages;
                gs_callstack    := new_stack;
                gs_context_u128 := zero128;
 
 
-               gs_storages     := storages;
-               gs_contract_code:= codes;
+               gs_depot        := depot;
+               gs_contracts    := codes;
              |}
 
 
 |step_FarCall_NonKernel_HeapOrAuxHeap:
-  forall flags regs mem_pages xstack0 xstack1 xstack2 
-                                   (handler:imm_in) handler_location storages
+  forall flags regs pages xstack0 xstack1 xstack2 
+                                   (handler:imm_in) handler_location depot
                                    codes context_u128 (abi dest:in_reg)
-                                   is_static new_mem_pages
+                                   is_static new_pages
                                    new_code_page (dest_val:word_type)
                                    abi_val
                                    new_mem_ctx in_ptr shard_id
@@ -212,11 +213,11 @@ Inductive step_farcall: instruction -> global_state -> global_state -> Prop :=
                                    pass_ergs_actual ,
 
     let old_extframe := topmost_extframe xstack0 in
-    let old_mem_ctx  := old_extframe.(ecf_mem_context) in
+    let old_mem_ctx  := old_extframe.(ecf_pages) in
     let current_contract := old_extframe.(ecf_this_address) in
-    resolve_fetch_value regs xstack0 mem_pages dest (mk_pv vtag dest_val) ->
-    resolve_fetch_value regs xstack0 mem_pages abi (PtrValue abi_val) ->
-    resolve_fetch_value regs xstack0 mem_pages handler (IntValue handler_location) ->
+    resolve_fetch_value regs xstack0 pages dest (mk_pv vtag dest_val) ->
+    resolve_fetch_value regs xstack0 pages abi (PtrValue abi_val) ->
+    resolve_fetch_value regs xstack0 pages handler (IntValue handler_location) ->
     let dest_addr := resize _ 160 dest_val in
 
     addr_is_kernel dest_addr = false ->
@@ -233,9 +234,9 @@ Inductive step_farcall: instruction -> global_state -> global_state -> Prop :=
     (fwd_mode = UseHeap \/ fwd_mode = UseAuxHeap) ->
     validate_fresh in_ptr = no_exceptions ->
     select_page_bound xstack0 fwd_mode (page_id, current_bound) ->
-    code_fetch_and_pay storages codes dest_addr xstack0 (xstack1, new_code_page) ->
+    code_fetch_and_pay depot codes dest_addr xstack0 (xstack1, new_code_page) ->
 
-    alloc_pages_extframe mem_pages old_extframe.(ecf_mem_context) new_code_page (new_mem_pages, new_mem_ctx) ->
+    alloc_pages_extframe pages old_extframe.(ecf_pages) new_code_page (new_pages, new_mem_ctx) ->
 
     fat_ptr_induced_growth in_ptr current_bound diff ->
     pay (Ergs.growth_cost diff) xstack1 xstack2 ->
@@ -245,17 +246,17 @@ Inductive step_farcall: instruction -> global_state -> global_state -> Prop :=
 
     pass_allowed_ergs pass_ergs_query pass_ergs_actual xstack3 new_caller_stack ->
 
-    let out_ptr := in_ptr <| fp_mem_page := page_id |> in
+    let out_ptr := in_ptr <| fp_page := page_id |> in
     let new_regs := regs_state_zero <| gprs_r1 := PtrValue (FatPointer.ABI.(encode) out_ptr) |> in
     let new_xstack := ExternalCall {|
                       ecf_this_address := dest_addr;
                       ecf_msg_sender := current_contract;
                       ecf_code_address := zero16;
-                      ecf_mem_context := new_mem_ctx;
+                      ecf_pages       := new_mem_ctx;
                       ecf_is_static :=  ecf_is_static old_extframe || is_static;
                       ecf_context_u128_value := context_u128;
-                      ecf_saved_storage_state := load _ current_contract storages;
-                      ecx_common := {|
+                      ecf_saved_storage_state := load _ current_contract depot;
+                      ecf_common := {|
                                      cf_exception_handler_location := resize _ _ handler_location;
                                      cf_sp := INITIAL_SP_ON_FAR_CALL;
                                      cf_pc := zero16;
@@ -267,24 +268,104 @@ Inductive step_farcall: instruction -> global_state -> global_state -> Prop :=
              {|
                gs_flags        := flags;
                gs_regs         := regs;
-               gs_mem_pages    := mem_pages;
+               gs_pages    := pages;
                gs_callstack    := xstack0;
                gs_context_u128 := context_u128;
 
 
-               gs_storages    := storages;
-               gs_contract_code:= codes;
+               gs_depot    := depot;
+               gs_contracts    := codes;
              |}
              {|
                gs_flags        := flags_clear;
                gs_regs         := new_regs;
-               gs_mem_pages    := new_mem_pages;
+               gs_pages    := new_pages;
                gs_callstack    := new_xstack;
                gs_context_u128 := zero128;
 
 
-               gs_storages     := storages;
-               gs_contract_code:= codes;
+               gs_depot     := depot;
+               gs_contracts    := codes;
              |}
+
+|step_FarCall_Kernel_Forward: forall flags regs pages xstack0 xstack1 xstack2
+                                   (handler:imm_in) handler_location depot
+                                   codes context_u128 (abi dest:in_reg)
+                                   is_static new_pages
+                                   new_code_page (dest_val:word_type)
+                                   abi_val
+                                   new_mem_ctx in_ptr shrunk_ptr shard_id
+                                   pass_ergs_query pass_ergs_actual vtag,
+
+    let old_extframe := topmost_extframe xstack0 in
+    let old_mem_ctx  := old_extframe.(ecf_pages) in
+    let current_contract := old_extframe.(ecf_this_address) in
+
+    resolve_fetch_value regs xstack0 pages dest (mk_pv vtag dest_val) ->
+    resolve_fetch_value regs xstack0 pages abi (PtrValue abi_val) ->
+    resolve_fetch_value regs xstack0 pages handler (IntValue handler_location) ->
+    let dest_addr := resize _ 160 dest_val in
+    addr_is_kernel dest_addr = true ->
+    
+    FarCall.ABI.(decode) abi_val = Some
+                                     {|
+                                       fc_memory_quasi_fat_ptr := in_ptr;
+                                       fc_ergs_passed := pass_ergs_query;
+                                       fc_shard_id := shard_id;
+                                       fc_forwarding_mode := ForwardFatPointer;
+                                       fc_constructor_call := false;
+                                       fc_to_system := true;
+                                     |} ->
+
+    fat_ptr_shrink in_ptr shrunk_ptr ->
+
+    code_fetch_and_pay depot codes dest_addr xstack0 (xstack1, new_code_page) ->
+
+    alloc_pages_extframe pages old_mem_ctx new_code_page (new_pages, new_mem_ctx) ->
+
+    pass_allowed_ergs pass_ergs_query pass_ergs_actual xstack1 xstack2 ->
+
+    let encoded_shrunk_ptr := FatPointer.ABI.(encode) shrunk_ptr in
+    let new_regs := regs_state_zero <| gprs_r1 := PtrValue encoded_shrunk_ptr |> in
+    let new_stack := ExternalCall {|
+                         ecf_this_address := dest_addr;
+                         ecf_msg_sender := current_contract;
+                         ecf_code_address := zero16;
+                         ecf_pages       := new_mem_ctx;
+                         ecf_is_static :=  ecf_is_static old_extframe || is_static;
+                         ecf_context_u128_value := context_u128;
+                         ecf_saved_storage_state := load _ current_contract depot;
+                         ecf_common := {|
+                                        cf_exception_handler_location
+                                        := resize _ code_address_bits handler_location;
+                                        cf_sp := INITIAL_SP_ON_FAR_CALL;
+                                        cf_pc := zero16;
+                                        cf_ergs_remaining := pass_ergs_actual;
+                                      |};
+                       |} (Some xstack2) in
+    step_farcall (OpFarCall abi dest handler is_static)
+             {|
+               gs_flags        := flags;
+               gs_regs         := regs;
+               gs_pages    := pages;
+               gs_callstack    := xstack0;
+               gs_context_u128 := context_u128;
+
+
+               gs_depot     := depot;
+               gs_contracts    := codes;
+             |}
+             {|
+               gs_flags        := flags_clear;
+               gs_regs         := new_regs;
+               gs_pages        := new_pages;
+               gs_callstack    := new_stack;
+               gs_context_u128 := zero128;
+
+
+               gs_depot        := depot;
+               gs_contracts    := codes;
+             |}
+
 
 .
