src/MemoryOps.v
@@ -1,6 +1,6 @@
-Require Common Condition Memory Instruction State.
+Require Common Condition ExecutionStack Memory Instruction State.
 
-Import ZArith ZMod Common Condition MemoryBase Memory Instruction State Arg List ListNotations.
+Import ZArith ZMod Common Condition ExecutionStack MemoryBase Memory Instruction State Arg List ListNotations.
 
 (** Location from where a value can be fetched. *)
 Inductive loc : Set :=
@@ -9,12 +9,12 @@ Inductive loc : Set :=
 | LocStackAddress: stack_address -> loc
 | LocCodeAddr: code_address -> loc
 | LocConstAddr: const_address ->  loc
-| LocHeapAddr: mem_page_id -> mem_address -> loc
-| LocAuxHeapAddr: mem_page_id -> mem_address ->  loc.
+| LocHeapAddr: page_id -> mem_address -> loc
+| LocAuxHeapAddr: page_id -> mem_address ->  loc.
 
 
 Section GPR.
-(** Fetching value from general purpose register. *)
+  (** Fetching value from general purpose register. *)
 
   Definition fetch_gpr (rs:regs_state) (r:reg_name) : primitive_value :=
     match r with
@@ -36,292 +36,276 @@ Section GPR.
     | R15 => gprs_r15 rs
     end.
 
-(** Storing value to general purpose registers. *)
-
-
-
-(** Storing value to general purpose registers. *)
-Inductive store_gpr : regs_state -> reg_name -> primitive_value -> regs_state -> Prop :=
-| fr_store1 :
-  forall r1 r2 r3 r4 r5 r6 r7 r8 r9 r10 r11 r12 r13 r14 r15 pv,
-  store_gpr
-    (mk_regs r1 r2 r3 r4 r5 r6 r7 r8 r9 r10 r11 r12 r13 r14 r15) R1 pv
-    (mk_regs pv r2 r3 r4 r5 r6 r7 r8 r9 r10 r11 r12 r13 r14 r15)
-| fr_store2 :
-  forall r1 r2 r3 r4 r5 r6 r7 r8 r9 r10 r11 r12 r13 r14 r15 pv,
-  store_gpr
-    (mk_regs r1 r2 r3 r4 r5 r6 r7 r8 r9 r10 r11 r12 r13 r14 r15) R2 pv
-    (mk_regs r1 pv r3 r4 r5 r6 r7 r8 r9 r10 r11 r12 r13 r14 r15)
-| fr_store3 :
-  forall r1 r2 r3 r4 r5 r6 r7 r8 r9 r10 r11 r12 r13 r14 r15 pv,
-  store_gpr
-    (mk_regs r1 r2 r3 r4 r5 r6 r7 r8 r9 r10 r11 r12 r13 r14 r15) R3 pv
-    (mk_regs r1 r2 pv r4 r5 r6 r7 r8 r9 r10 r11 r12 r13 r14 r15)
-| fr_store4 :
-  forall r1 r2 r3 r4 r5 r6 r7 r8 r9 r10 r11 r12 r13 r14 r15 pv,
-  store_gpr
-    (mk_regs r1 r2 r3 r4 r5 r6 r7 r8 r9 r10 r11 r12 r13 r14 r15) R4 pv
-    (mk_regs r1 r2 r3 pv r5 r6 r7 r8 r9 r10 r11 r12 r13 r14 r15)
-| fr_store5 :
-  forall r1 r2 r3 r4 r5 r6 r7 r8 r9 r10 r11 r12 r13 r14 r15 pv,
-  store_gpr
-    (mk_regs r1 r2 r3 r4 r5 r6 r7 r8 r9 r10 r11 r12 r13 r14 r15) R5 pv
-    (mk_regs r1 r2 r3 r4 pv r6 r7 r8 r9 r10 r11 r12 r13 r14 r15)
-| fr_store6 :
-  forall r1 r2 r3 r4 r5 r6 r7 r8 r9 r10 r11 r12 r13 r14 r15 pv,
-    store_gpr
-      (mk_regs r1 r2 r3 r4 r5 r6 r7 r8 r9 r10 r11 r12 r13 r14 r15) R6 pv
-      (mk_regs r1 r2 r3 r4 r5 pv r7 r8 r9 r10 r11 r12 r13 r14 r15)
-| fr_store7 :
-  forall r1 r2 r3 r4 r5 r6 r7 r8 r9 r10 r11 r12 r13 r14 r15 pv,
-    store_gpr
-      (mk_regs r1 r2 r3 r4 r5 r6 r7 r8 r9 r10 r11 r12 r13 r14 r15) R7 pv
-      (mk_regs r1 r2 r3 r4 r5 r6 pv r8 r9 r10 r11 r12 r13 r14 r15)
-| fr_store8 :
-  forall r1 r2 r3 r4 r5 r6 r7 r8 r9 r10 r11 r12 r13 r14 r15 pv,
-    store_gpr
-      (mk_regs r1 r2 r3 r4 r5 r6 r7 r8 r9 r10 r11 r12 r13 r14 r15) R8 pv
-      (mk_regs r1 r2 r3 r4 r5 r6 r7 pv r9 r10 r11 r12 r13 r14 r15)
-| fr_store9 :
-  forall r1 r2 r3 r4 r5 r6 r7 r8 r9 r10 r11 r12 r13 r14 r15 pv,
-    store_gpr
-      (mk_regs r1 r2 r3 r4 r5 r6 r7 r8 r9 r10 r11 r12 r13 r14 r15) R9 pv
-      (mk_regs r1 r2 r3 r4 r5 r6 r7 r8 pv r10 r11 r12 r13 r14 r15)
-| fr_store10 :
-  forall r1 r2 r3 r4 r5 r6 r7 r8 r9 r10 r11 r12 r13 r14 r15 pv,
-    store_gpr
-      (mk_regs r1 r2 r3 r4 r5 r6 r7 r8 r9 r10 r11 r12 r13 r14 r15) R10 pv
-      (mk_regs r1 r2 r3 r4 r5 r6 r7 r8 r9 pv r11 r12 r13 r14 r15)
-| fr_store11 :
-  forall r1 r2 r3 r4 r5 r6 r7 r8 r9 r10 r11 r12 r13 r14 r15 pv,
-    store_gpr
-      (mk_regs r1 r2 r3 r4 r5 r6 r7 r8 r9 r10 r11 r12 r13 r14 r15) R11 pv
-      (mk_regs r1 r2 r3 r4 r5 r6 r7 r8 r9 r10 pv r12 r13 r14 r15)
-| fr_store12 :
-  forall r1 r2 r3 r4 r5 r6 r7 r8 r9 r10 r11 r12 r13 r14 r15 pv,
-    store_gpr
-      (mk_regs r1 r2 r3 r4 r5 r6 r7 r8 r9 r10 r11 r12 r13 r14 r15) R12 pv
-      (mk_regs r1 r2 r3 r4 r5 r6 r7 r8 r9 r10 r11 pv r13 r14 r15)
-| fr_store13 :
-  forall r1 r2 r3 r4 r5 r6 r7 r8 r9 r10 r11 r12 r13 r14 r15 pv,
-    store_gpr
-      (mk_regs r1 r2 r3 r4 r5 r6 r7 r8 r9 r10 r11 r12 r13 r14 r15) R13 pv
-      (mk_regs r1 r2 r3 r4 r5 r6 r7 r8 r9 r10 r11 r12 pv r14 r15)
-| fr_store14 :
-  forall r1 r2 r3 r4 r5 r6 r7 r8 r9 r10 r11 r12 r13 r14 r15 pv,
-    store_gpr
-      (mk_regs r1 r2 r3 r4 r5 r6 r7 r8 r9 r10 r11 r12 r13 r14 r15) R14 pv
-      (mk_regs r1 r2 r3 r4 r5 r6 r7 r8 r9 r10 r11 r12 r13 pv r15)
-| fr_store15 :
-  forall r1 r2 r3 r4 r5 r6 r7 r8 r9 r10 r11 r12 r13 r14 r15 pv,
-    store_gpr
-      (mk_regs r1 r2 r3 r4 r5 r6 r7 r8 r9 r10 r11 r12 r13 r14 r15) R15 pv
-      (mk_regs r1 r2 r3 r4 r5 r6 r7 r8 r9 r10 r11 r12 r13 r14 pv)
-.
+  (** Storing value to general purpose registers. *)
+  Inductive store_gpr : regs_state -> reg_name -> primitive_value -> regs_state -> Prop :=
+  | fr_store1 :
+    forall r1 r2 r3 r4 r5 r6 r7 r8 r9 r10 r11 r12 r13 r14 r15 pv,
+      store_gpr
+        (mk_regs r1 r2 r3 r4 r5 r6 r7 r8 r9 r10 r11 r12 r13 r14 r15) R1 pv
+        (mk_regs pv r2 r3 r4 r5 r6 r7 r8 r9 r10 r11 r12 r13 r14 r15)
+  | fr_store2 :
+    forall r1 r2 r3 r4 r5 r6 r7 r8 r9 r10 r11 r12 r13 r14 r15 pv,
+      store_gpr
+        (mk_regs r1 r2 r3 r4 r5 r6 r7 r8 r9 r10 r11 r12 r13 r14 r15) R2 pv
+        (mk_regs r1 pv r3 r4 r5 r6 r7 r8 r9 r10 r11 r12 r13 r14 r15)
+  | fr_store3 :
+    forall r1 r2 r3 r4 r5 r6 r7 r8 r9 r10 r11 r12 r13 r14 r15 pv,
+      store_gpr
+        (mk_regs r1 r2 r3 r4 r5 r6 r7 r8 r9 r10 r11 r12 r13 r14 r15) R3 pv
+        (mk_regs r1 r2 pv r4 r5 r6 r7 r8 r9 r10 r11 r12 r13 r14 r15)
+  | fr_store4 :
+    forall r1 r2 r3 r4 r5 r6 r7 r8 r9 r10 r11 r12 r13 r14 r15 pv,
+      store_gpr
+        (mk_regs r1 r2 r3 r4 r5 r6 r7 r8 r9 r10 r11 r12 r13 r14 r15) R4 pv
+        (mk_regs r1 r2 r3 pv r5 r6 r7 r8 r9 r10 r11 r12 r13 r14 r15)
+  | fr_store5 :
+    forall r1 r2 r3 r4 r5 r6 r7 r8 r9 r10 r11 r12 r13 r14 r15 pv,
+      store_gpr
+        (mk_regs r1 r2 r3 r4 r5 r6 r7 r8 r9 r10 r11 r12 r13 r14 r15) R5 pv
+        (mk_regs r1 r2 r3 r4 pv r6 r7 r8 r9 r10 r11 r12 r13 r14 r15)
+  | fr_store6 :
+    forall r1 r2 r3 r4 r5 r6 r7 r8 r9 r10 r11 r12 r13 r14 r15 pv,
+      store_gpr
+        (mk_regs r1 r2 r3 r4 r5 r6 r7 r8 r9 r10 r11 r12 r13 r14 r15) R6 pv
+        (mk_regs r1 r2 r3 r4 r5 pv r7 r8 r9 r10 r11 r12 r13 r14 r15)
+  | fr_store7 :
+    forall r1 r2 r3 r4 r5 r6 r7 r8 r9 r10 r11 r12 r13 r14 r15 pv,
+      store_gpr
+        (mk_regs r1 r2 r3 r4 r5 r6 r7 r8 r9 r10 r11 r12 r13 r14 r15) R7 pv
+        (mk_regs r1 r2 r3 r4 r5 r6 pv r8 r9 r10 r11 r12 r13 r14 r15)
+  | fr_store8 :
+    forall r1 r2 r3 r4 r5 r6 r7 r8 r9 r10 r11 r12 r13 r14 r15 pv,
+      store_gpr
+        (mk_regs r1 r2 r3 r4 r5 r6 r7 r8 r9 r10 r11 r12 r13 r14 r15) R8 pv
+        (mk_regs r1 r2 r3 r4 r5 r6 r7 pv r9 r10 r11 r12 r13 r14 r15)
+  | fr_store9 :
+    forall r1 r2 r3 r4 r5 r6 r7 r8 r9 r10 r11 r12 r13 r14 r15 pv,
+      store_gpr
+        (mk_regs r1 r2 r3 r4 r5 r6 r7 r8 r9 r10 r11 r12 r13 r14 r15) R9 pv
+        (mk_regs r1 r2 r3 r4 r5 r6 r7 r8 pv r10 r11 r12 r13 r14 r15)
+  | fr_store10 :
+    forall r1 r2 r3 r4 r5 r6 r7 r8 r9 r10 r11 r12 r13 r14 r15 pv,
+      store_gpr
+        (mk_regs r1 r2 r3 r4 r5 r6 r7 r8 r9 r10 r11 r12 r13 r14 r15) R10 pv
+        (mk_regs r1 r2 r3 r4 r5 r6 r7 r8 r9 pv r11 r12 r13 r14 r15)
+  | fr_store11 :
+    forall r1 r2 r3 r4 r5 r6 r7 r8 r9 r10 r11 r12 r13 r14 r15 pv,
+      store_gpr
+        (mk_regs r1 r2 r3 r4 r5 r6 r7 r8 r9 r10 r11 r12 r13 r14 r15) R11 pv
+        (mk_regs r1 r2 r3 r4 r5 r6 r7 r8 r9 r10 pv r12 r13 r14 r15)
+  | fr_store12 :
+    forall r1 r2 r3 r4 r5 r6 r7 r8 r9 r10 r11 r12 r13 r14 r15 pv,
+      store_gpr
+        (mk_regs r1 r2 r3 r4 r5 r6 r7 r8 r9 r10 r11 r12 r13 r14 r15) R12 pv
+        (mk_regs r1 r2 r3 r4 r5 r6 r7 r8 r9 r10 r11 pv r13 r14 r15)
+  | fr_store13 :
+    forall r1 r2 r3 r4 r5 r6 r7 r8 r9 r10 r11 r12 r13 r14 r15 pv,
+      store_gpr
+        (mk_regs r1 r2 r3 r4 r5 r6 r7 r8 r9 r10 r11 r12 r13 r14 r15) R13 pv
+        (mk_regs r1 r2 r3 r4 r5 r6 r7 r8 r9 r10 r11 r12 pv r14 r15)
+  | fr_store14 :
+    forall r1 r2 r3 r4 r5 r6 r7 r8 r9 r10 r11 r12 r13 r14 r15 pv,
+      store_gpr
+        (mk_regs r1 r2 r3 r4 r5 r6 r7 r8 r9 r10 r11 r12 r13 r14 r15) R14 pv
+        (mk_regs r1 r2 r3 r4 r5 r6 r7 r8 r9 r10 r11 r12 r13 pv r15)
+  | fr_store15 :
+    forall r1 r2 r3 r4 r5 r6 r7 r8 r9 r10 r11 r12 r13 r14 r15 pv,
+      store_gpr
+        (mk_regs r1 r2 r3 r4 r5 r6 r7 r8 r9 r10 r11 r12 r13 r14 r15) R15 pv
+        (mk_regs r1 r2 r3 r4 r5 r6 r7 r8 r9 r10 r11 r12 r13 r14 pv)
+  .
 
 End GPR.
 
+Section Addressing.
 
-Section AddressResolution.
-Inductive reg_rel_addressing addr_bits : regs_state -> reg_name -> int_mod addr_bits -> int_mod addr_bits -> Prop :=
-| rca_code_pp: forall regs reg reg_val base ofs
-                 abs OF_ignored,
-    fetch_gpr regs reg = IntValue reg_val ->
-    extract_address addr_bits reg_val base ->
-    uadd_overflow _ base ofs = (abs, OF_ignored) ->
-    reg_rel_addressing addr_bits regs reg ofs abs.
+  Inductive reg_rel addr_bits : regs_state -> reg_name -> int_mod addr_bits -> int_mod addr_bits -> Prop :=
+  | rca_code_pp: forall regs reg reg_val base ofs
+                   abs OF_ignored,
+      fetch_gpr regs reg = IntValue reg_val ->
+      extract_address addr_bits reg_val base ->
+      base + ofs = (abs, OF_ignored) ->
+      reg_rel addr_bits regs reg ofs abs.
 
-Definition reg_rel_code_addressing
-  : regs_state -> reg_name -> u16 -> code_address -> Prop
-  := reg_rel_addressing code_address_bits.
+  Definition reg_rel_code : regs_state -> reg_name -> u16 -> code_address -> Prop
+    := reg_rel code_address_bits.
 
-Definition reg_rel_const_addressing
-  : regs_state -> reg_name -> u16 -> const_address -> Prop
-  := reg_rel_addressing const_address_bits.
+  Definition reg_rel_const
+    : regs_state -> reg_name -> u16 -> const_address -> Prop
+    := reg_rel const_address_bits.
 
-Definition reg_rel_stack_addressing
-  : regs_state -> reg_name -> u16 -> stack_address -> Prop
-  := reg_rel_addressing stack_page_params.(address_bits).
+  Definition reg_rel_stack
+    : regs_state -> reg_name -> u16 -> stack_address -> Prop
+    := reg_rel stack_page_params.(address_bits).
 
-(** delta = reg + imm *)
-Definition sp_delta_abs: regs_state -> reg_name -> u16 -> stack_address -> Prop := reg_rel_stack_addressing.
+  (** delta = reg + imm *)
+  Definition sp_delta_abs: regs_state -> reg_name -> u16 -> stack_address -> Prop := reg_rel_stack.
 
 
-Inductive loc_reg: reg_io -> loc ->  Prop :=
-| rslv_reg_aux: forall reg, loc_reg (Reg reg) (LocReg reg).
+  Inductive loc_reg: reg_io -> loc ->  Prop :=
+  | rslv_reg_aux: forall reg, loc_reg (Reg reg) (LocReg reg).
 
-Inductive loc_imm: imm_in -> loc ->  Prop :=
-|rslv_imm_aux : forall imm, loc_imm (Imm imm) (LocImm imm).
+  Inductive loc_imm: imm_in -> loc ->  Prop :=
+  |rslv_imm_aux : forall imm, loc_imm (Imm imm) (LocImm imm).
 
-Inductive loc_code: regs_state -> code_in -> loc -> Prop :=
-| rslv_code_aux: forall regs reg abs_imm addr,
-    reg_rel_code_addressing regs reg abs_imm addr ->
-    loc_code regs (CodeAddr reg abs_imm) (LocCodeAddr addr).
+  Inductive loc_code: regs_state -> code_in -> loc -> Prop :=
+  | rslv_code_aux: forall regs reg abs_imm addr,
+      reg_rel_code regs reg abs_imm addr ->
+      loc_code regs (CodeAddr reg abs_imm) (LocCodeAddr addr).
 
-Inductive loc_const: regs_state -> const_in -> loc -> Prop :=
-| rslv_const_aux: forall regs reg abs_imm addr,
-    reg_rel_const_addressing regs reg abs_imm addr ->
-    loc_const regs (ConstAddr reg abs_imm) (LocConstAddr addr).
+  Inductive loc_const: regs_state -> const_in -> loc -> Prop :=
+  | rslv_const_aux: forall regs reg abs_imm addr,
+      reg_rel_const regs reg abs_imm addr ->
+      loc_const regs (ConstAddr reg abs_imm) (LocConstAddr addr).
 
-Inductive loc_stack_io: execution_frame -> regs_state -> stack_io -> loc -> Prop :=
-| rslv_stack_rel_aux: forall ef regs reg base offset_imm dlt_sp sp_rel OF_ignore,
-    fetch_sp ef base ->
-    sp_delta_abs regs reg offset_imm dlt_sp ->
-    (sp_rel, OF_ignore) = usub_overflow _ base dlt_sp->
-    loc_stack_io ef regs (RelSP reg offset_imm) (LocStackAddress sp_rel)
-| rslv_stack_abs_aux: forall ef regs reg imm abs,
-    reg_rel_stack_addressing regs reg imm abs ->
-    loc_stack_io ef regs (Absolute reg imm) (LocStackAddress imm).
+  Inductive loc_stack_io: execution_stack -> regs_state -> stack_io -> loc -> Prop :=
+  | rslv_stack_rel_aux: forall ef regs reg offset_imm dlt_sp sp_rel OF_ignore,
+      let base := sp_get ef in
+      sp_delta_abs regs reg offset_imm dlt_sp ->
+      (sp_rel, OF_ignore) = usub_overflow _ base dlt_sp->
+      loc_stack_io ef regs (RelSP reg offset_imm) (LocStackAddress sp_rel)
+  | rslv_stack_abs_aux: forall ef regs reg imm abs,
+      reg_rel_stack regs reg imm abs ->
+      loc_stack_io ef regs (Absolute reg imm) (LocStackAddress imm).
 
-Inductive loc_stack_in_only: execution_frame -> regs_state -> stack_in_only -> loc -> Prop :=
-| rslv_stack_gpop_aux: forall ef regs reg sp ofs dlt_sp new_sp OF_ignore,
-    fetch_sp ef sp ->
-    sp_delta_abs regs reg ofs dlt_sp ->
-    (new_sp, OF_ignore) = usub_overflow _ sp dlt_sp ->
-    loc_stack_in_only ef regs (RelSpPop reg ofs) (LocStackAddress new_sp)
-.
+  Inductive loc_stack_in_only: execution_stack -> regs_state -> stack_in_only -> loc -> Prop :=
+  | rslv_stack_gpop_aux: forall ef regs reg ofs dlt_sp new_sp OF_ignore,
+      let sp := sp_get ef in
+      sp_delta_abs regs reg ofs dlt_sp ->
+      (new_sp, OF_ignore) = usub_overflow _ sp dlt_sp ->
+      loc_stack_in_only ef regs (RelSpPop reg ofs) (LocStackAddress new_sp)
+  .
 
-Inductive loc_stack_out_only: execution_frame -> regs_state -> stack_out_only -> loc -> Prop :=
-| rslv_stack_gpush_aux: forall ef regs reg sp ofs dlt_sp new_sp OF_ignore,
-    fetch_sp ef sp ->
-    sp_delta_abs regs reg ofs dlt_sp ->
-    (new_sp, OF_ignore) = uadd_overflow _ sp dlt_sp ->
-    loc_stack_out_only ef regs (RelSpPush reg ofs) (LocStackAddress new_sp)
-.
+  Inductive loc_stack_out_only: execution_stack -> regs_state -> stack_out_only -> loc -> Prop :=
+  | rslv_stack_gpush_aux: forall ef regs reg ofs dlt_sp new_sp OF_ignore,
+      let sp := sp_get ef in
+      sp_delta_abs regs reg ofs dlt_sp ->
+      (new_sp, OF_ignore) = sp + dlt_sp ->
+      loc_stack_out_only ef regs (RelSpPush reg ofs) (LocStackAddress new_sp)
+  .
 
-Inductive resolve: execution_frame -> regs_state -> any -> loc -> Prop :=
-| rslv_reg : forall ef rs r loc,
-    loc_reg r loc ->
-    resolve ef rs (AnyReg r) loc
-| rslv_imm: forall ef rs imm loc,
-    loc_imm imm loc ->
-    resolve ef rs (AnyImm imm) loc
-| rslv_stack_io: forall ef regs arg loc,
-    loc_stack_io ef regs arg loc ->
-    resolve ef regs (AnyStack (StackAnyIO arg)) loc
-| rslv_stack_in: forall ef regs arg loc,
-    loc_stack_in_only ef regs arg loc ->
-    resolve ef regs (AnyStack (StackAnyIn arg)) loc
-| rslv_stack_out: forall ef regs arg loc,
-    loc_stack_out_only ef regs arg loc ->
-    resolve ef regs (AnyStack (StackAnyOut arg)) loc
-| rslv_code: forall ef regs arg loc,
-    loc_code regs arg loc ->
-    resolve ef regs (AnyCode arg) loc
-| rslv_const: forall ef regs arg loc,
-    loc_const regs arg loc ->
-    resolve ef regs (AnyConst arg) loc
-.
+  Inductive resolve: execution_stack -> regs_state -> any -> loc -> Prop :=
+  | rslv_reg : forall ef rs r loc,
+      loc_reg r loc ->
+      resolve ef rs (AnyReg r) loc
+  | rslv_imm: forall ef rs imm loc,
+      loc_imm imm loc ->
+      resolve ef rs (AnyImm imm) loc
+  | rslv_stack_io: forall ef regs arg loc,
+      loc_stack_io ef regs arg loc ->
+      resolve ef regs (AnyStack (StackAnyIO arg)) loc
+  | rslv_stack_in: forall ef regs arg loc,
+      loc_stack_in_only ef regs arg loc ->
+      resolve ef regs (AnyStack (StackAnyIn arg)) loc
+  | rslv_stack_out: forall ef regs arg loc,
+      loc_stack_out_only ef regs arg loc ->
+      resolve ef regs (AnyStack (StackAnyOut arg)) loc
+  | rslv_code: forall ef regs arg loc,
+      loc_code regs arg loc ->
+      resolve ef regs (AnyCode arg) loc
+  | rslv_const: forall ef regs arg loc,
+      loc_const regs arg loc ->
+      resolve ef regs (AnyConst arg) loc
+  .
 
-Inductive resolve_effect__in: in_any -> execution_frame -> execution_frame -> Prop :=
-| rslv_stack_in_effect: forall ef ef' regs sp' reg ofs arg,
-    loc_stack_in_only ef regs  arg (LocStackAddress sp') ->
-    update_sp sp' ef ef' ->
-    resolve_effect__in  (InStack (StackInOnly (RelSpPop reg ofs)))  ef ef'
-| rslv_stack_in_effect_none: forall ef arg,
-    (forall reg ofs, arg <> InStack (StackInOnly (RelSpPop reg ofs))) ->
-    resolve_effect__in  arg  ef ef.
+  Inductive resolve_effect__in: in_any -> execution_stack -> execution_stack -> Prop :=
+  | rslv_stack_in_effect: forall ef regs sp' reg ofs arg,
+      loc_stack_in_only ef regs  arg (LocStackAddress sp') ->
+      let ef' := sp_update sp' ef in
+      resolve_effect__in  (InStack (StackInOnly (RelSpPop reg ofs)))  ef ef'
+  | rslv_stack_in_effect_none: forall ef arg,
+      (forall reg ofs, arg <> InStack (StackInOnly (RelSpPop reg ofs))) ->
+      resolve_effect__in  arg  ef ef.
 
-Inductive resolve_effect__out: out_any -> execution_frame -> execution_frame -> Prop :=
-| rslv_stack_out_effect: forall ef ef' regs sp' reg ofs arg,
-    loc_stack_out_only ef regs  arg (LocStackAddress sp') ->
-    update_sp sp' ef ef' ->
-    resolve_effect__out  (OutStack (StackOutOnly (RelSpPush reg ofs)))  ef ef'
-| rslv_stack_out_effect_none: forall ef arg,
-    (forall reg ofs, arg <> OutStack (StackOutOnly (RelSpPush reg ofs))) ->
-    resolve_effect__out  arg  ef ef.
+  Inductive resolve_effect__out: out_any -> execution_stack -> execution_stack -> Prop :=
+  | rslv_stack_out_effect: forall ef regs sp' reg ofs arg,
+      loc_stack_out_only ef regs  arg (LocStackAddress sp') ->
+      let ef' := sp_update sp' ef in
+      resolve_effect__out  (OutStack (StackOutOnly (RelSpPush reg ofs)))  ef ef'
+  | rslv_stack_out_effect_none: forall ef arg,
+      (forall reg ofs, arg <> OutStack (StackOutOnly (RelSpPush reg ofs))) ->
+      resolve_effect__out  arg  ef ef.
 
-Inductive resolve_effect: in_any -> out_any -> execution_frame -> execution_frame -> Prop :=
-| rslv_effect_full: forall arg1 arg2 ef1 ef2 ef3,
-    resolve_effect__in arg1 ef1 ef2 ->
-    resolve_effect__out arg2 ef2 ef3 ->
-    resolve_effect arg1 arg2 ef1 ef3.
+  Inductive resolve_effect: in_any -> out_any -> execution_stack -> execution_stack -> Prop :=
+  | rslv_effect_full: forall arg1 arg2 ef1 ef2 ef3,
+      resolve_effect__in arg1 ef1 ef2 ->
+      resolve_effect__out arg2 ef2 ef3 ->
+      resolve_effect arg1 arg2 ef1 ef3.
 
-End AddressResolution.
+End Addressing.
 
 Section FetchStore.
 
-Inductive fetch_result : Set :=
-| FetchIns (ins :instruction_predicated)
-| FetchPV (pv: primitive_value) .
+  Inductive fetch_result : Set :=
+  | FetchIns (ins :instruction_predicated)
+  | FetchPV (pv: primitive_value) .
 
-(* Address resolution *)
-Inductive fetch_loc: regs_state -> execution_frame -> mem_manager -> loc -> fetch_result -> Prop :=
-| fetch_reg:
-  forall regs ef mm reg_name value,
-    fetch_gpr regs reg_name = value ->
-    fetch_loc regs ef mm (LocReg reg_name) (FetchPV value)
+  (* Address resolution *)
+  Inductive fetch_loc: regs_state -> execution_stack -> pages -> loc -> fetch_result -> Prop :=
+  | fetch_reg:
+    forall regs ef mm reg_name,
+      fetch_loc regs ef mm (LocReg reg_name) (FetchPV (fetch_gpr regs reg_name))
 
-| fetch_imm:
-  forall regs ef mm imm imm',
-    imm' = resize _ word_bits imm ->
-    fetch_loc regs ef mm (LocImm imm) (FetchPV (IntValue imm'))
+  | fetch_imm:
+    forall regs ef mm imm imm',
+      imm' = resize _ word_bits imm ->
+      fetch_loc regs ef mm (LocImm imm) (FetchPV (IntValue imm'))
 
-| fetch_stackaddr:
-  forall regs ef mm stackpage addr value,
-    mem_page_by_id mm (active_stack_id ef) (StackPage _ _ stackpage) ->
-    load_result _ addr stackpage value ->
-    fetch_loc regs ef mm (LocStackAddress addr) (FetchPV value)
-| fetch_codeaddr:
-  forall regs ef mm codepage addr ins,
-    mem_page_by_id mm (active_stack_id ef) (CodePage _ _ codepage) ->
-    load_result _ addr codepage ins ->
-    fetch_loc regs ef mm (LocCodeAddr addr) (FetchIns ins)
-| fetch_constaddr:
-  forall regs ef mm constpage addr value,
-    mem_page_by_id mm (active_stack_id ef) (ConstPage _ _ constpage) ->
-    load_result _ addr constpage value ->
-    fetch_loc regs ef mm (LocConstAddr addr) (FetchPV (IntValue value))
+  | fetch_stackaddr:
+    forall regs ef ps stackpage addr value,
+      active_stackpage ps ef (StackPage _ _ stackpage) ->
+      load_result _ addr stackpage value ->
+      fetch_loc regs ef ps (LocStackAddress addr) (FetchPV value)
+  | fetch_codeaddr:
+    forall regs ef ps codepage addr ins,
+      active_codepage ps ef (CodePage _ _ codepage) ->
+      load_result _ addr codepage ins ->
+      fetch_loc regs ef ps (LocCodeAddr addr) (FetchIns ins)
+  | fetch_constaddr:
+    forall regs ef ps constpage addr value,
+      active_codepage ps ef (ConstPage _ _ constpage) ->
+      load_result _ addr constpage value ->
+      fetch_loc regs ef ps (LocConstAddr addr) (FetchPV (IntValue value))
 
-.
-(* TODO UMA; reading byte sequences is already implemented, see
+  .
+  (* TODO UMA; reading byte sequences is already implemented, see
   tests in MemoryBase.v *)
 
-Inductive fetch_instr : regs_state -> execution_frame -> mem_manager -> instruction_predicated -> Prop :=
-| fi_fetch: forall regs ef mm pc ins,
-    fetch_pc ef pc ->
-    fetch_loc regs ef mm (LocCodeAddr pc) (FetchIns ins) ->
-    fetch_instr regs ef mm ins.
+  Inductive fetch_instr : regs_state -> execution_stack -> pages -> instruction_predicated -> Prop :=
+  | fi_fetch: forall regs ef mm ins,
+      fetch_loc regs ef mm (LocCodeAddr (pc_get ef)) (FetchIns ins) ->
+      fetch_instr regs ef mm ins.
 
-Inductive fetch_op: regs_state -> execution_frame -> mem_manager -> instruction -> cond -> Prop :=
-| fo_fetch: forall regs ef mm op cond,
-    fetch_instr regs ef mm (Ins op cond) ->
-    fetch_op regs ef mm op cond.
+  Inductive store_loc: regs_state -> execution_stack -> pages -> primitive_value -> loc -> (regs_state * pages) -> Prop :=
+  | store_reg:
+    forall regs regs' ef mm reg_name value,
+      store_gpr regs reg_name value regs' ->
+      store_loc regs ef mm value (LocReg reg_name) (regs', mm)
 
+  | store_stackaddr:
+    forall regs ef ps ps' stackpage addr value pid stackpage',
+      active_stackpage ps ef (StackPage _ _ stackpage) ->
+      store_result _ addr stackpage value stackpage' ->
+      page_replace pid (StackPage _ _ stackpage') ps ps' ->
+      store_loc regs ef ps value (LocStackAddress addr) (regs, ps')
+  .
+  (* TODO UMA related *)
 
+  Inductive resolve_fetch_value: regs_state -> execution_stack -> pages -> Arg.any -> primitive_value -> Prop :=
+  | rf_resfetch_pv: forall ef mm regs arg loc res,
+      resolve ef regs arg loc ->
+      fetch_loc regs ef mm loc (FetchPV res) ->
+      resolve_fetch_value regs ef mm arg res.
 
-Inductive store_loc: regs_state -> execution_frame -> mem_manager
-                     -> primitive_value -> loc -> (regs_state * mem_manager ) -> Prop :=
-| store_reg:
-  forall regs regs' ef mm reg_name value,
-    store_gpr regs reg_name value regs' ->
-    store_loc regs ef mm value (LocReg reg_name) (regs', mm)
-
-| store_stackaddr:
-  forall regs ef mm mm' stackpage addr value pid stackpage',
-    active_stackpage mm ef (StackPage _ _ stackpage) ->
-    store_result _ addr stackpage value stackpage' ->
-    mem_page_replace mm pid (StackPage _ _ stackpage') mm' ->
-    store_loc regs ef mm value (LocStackAddress addr) (regs, mm')
-.
-(* TODO UMA related *)
-
-Inductive resolve_fetch_value: regs_state -> execution_frame -> mem_manager
-                               -> Arg.any -> primitive_value -> Prop :=
-| rf_resfetch_pv: forall ef mm regs arg loc res,
-    resolve ef regs arg loc ->
-    fetch_loc regs ef mm loc (FetchPV res) ->
-    resolve_fetch_value regs ef mm arg res.
-
-Inductive resolve_fetch_word: regs_state -> execution_frame -> mem_manager -> Arg.any -> word_type -> Prop :=
-| rf_resfetch_w: forall ef mm regs arg res,
-    resolve_fetch_value regs ef mm arg (IntValue res) ->
-    resolve_fetch_word regs ef mm arg res.
+  Inductive resolve_fetch_word: regs_state -> execution_stack -> pages -> Arg.any -> word_type -> Prop :=
+  | rf_resfetch_w: forall ef mm regs arg res,
+      resolve_fetch_value regs ef mm arg (IntValue res) ->
+      resolve_fetch_word regs ef mm arg res.
 
 
-Inductive resolve_store: regs_state -> execution_frame -> mem_manager
-                         -> Arg.out_any -> primitive_value -> regs_state * mem_manager
-                         -> Prop :=
+  Inductive resolve_store: regs_state -> execution_stack -> pages
+                           -> Arg.out_any -> primitive_value -> regs_state * pages
+                           -> Prop :=
   | rs_resstore: forall ef mm regs arg loc_out pv regs' mm',
       resolve ef regs (out_any_incl arg) loc_out ->
       store_loc regs ef mm pv loc_out (regs', mm') ->
